src/lib/GPU.Conditional.fst
@@ -6,43 +6,65 @@ open FStar.Tactics.V2
 
 let if_ (b: bool) (p: slprop): slprop = (cond b p emp)
 
+
+// REWRITE
+
+```pulse
+ghost fn if_rewrite_bool (b1 b2: bool) (#_: squash (b1 == b2)) (p: slprop)
+  requires if_ b1 p
+  ensures  if_ b2 p
+{ () }
+```
+
+```pulse
+ghost fn if_rewrite (#b: bool) (#p1 p2: slprop) (#e: (squash b -> squash (p1 == p2)))
+  requires if_ b p1
+  ensures  if_ b p2
+{
+  if b {
+    e ();
+    rewrite each p1 as p2;
+  } else {
+    ()
+  }
+}
+```
+
 // INTRODUCTION and ELIMINATION RULES
 
 ```pulse
-ghost fn if_intro_true (b: bool { b }) (p: slprop)
+ghost fn if_intro_true (p: slprop)
   requires p
-  ensures  if_ b p
+  ensures  if_ true p
 {
-  rewrite p as if_ b p;
+  rewrite p as if_ true p;
 }
 ```
 
 ```pulse
-ghost fn if_intro_false (b: bool { not b }) (p: slprop)
+ghost fn if_intro_false (p: slprop)
   requires emp
-  ensures  if_ b p
+  ensures  if_ false p
 {
-  rewrite emp as if_ b p;
+  rewrite emp as if_ false p;
 }
 ```
 
 ```pulse
-ghost fn if_elim_true (b: bool { b }) (p: slprop)
-  requires if_ b p
+ghost fn if_elim_true (p: slprop)
+  requires if_ true p
   ensures  p
 {
-  unfold if_ b p;
-  rewrite (if b then p else emp) as p;
+  rewrite if_ true p as p;
 }
 ```
 
 ```pulse
-ghost fn if_elim_false (b: bool { not b }) (p: slprop)
-  requires if_ b p
+ghost fn if_elim_false (p: slprop)
+  requires if_ false p
   ensures  emp
 {
-  unfold if_ b p;
-  rewrite (if b then p else emp) as emp;
+  rewrite if_ false p as emp;
 }
 ```
 
@@ -54,11 +76,15 @@ ghost fn case_split (b: bool) (p: slprop)
   ensures  if_ b p ** if_ (not b) p
 {
   if b {
-    if_intro_true b p;
-    if_intro_false (not b) p;
+    if_intro_true p;
+    if_rewrite_bool true b p;
+    if_intro_false p;
+    if_rewrite_bool false (not b) p;
   } else {
-    if_intro_true (not b) p;
-    if_intro_false b p;
+    if_intro_true p;
+    if_rewrite_bool true (not b) p;
+    if_intro_false p;
+    if_rewrite_bool false b p;
   }
 }
 ```
@@ -69,12 +95,11 @@ ghost fn case_join (b: bool) (p: slprop)
   ensures  p
 {
   if b {
-    if_elim_true b p;
-    if_elim_false (not b) p;
+    if_elim_true p;
+    if_elim_false p;
   } else {
-    if_elim_true (not b) p;
-    if_elim_false b p;
-  
+    if_elim_true p;
+    if_elim_false p;
   }
 }
 ```
@@ -87,14 +112,13 @@ ghost fn combine (b: bool) (p1 p2: slprop)
   ensures  if_ b (p1 ** p2)
 {
   if b {
-    if_elim_true b p1;
-    if_elim_true b p2;
-    if_intro_true b (p1 ** p2);
+    if_elim_true p1;
+    if_elim_true p2;
+    if_intro_true (p1 ** p2);
   } else {
-    (* Why the assymetry here? using `b` fails *)
-    if_elim_false false p1;
-    if_elim_false false p2;
-    if_intro_false b (p1 ** p2);
+    if_elim_false p1;
+    if_elim_false p2;
+    if_intro_false (p1 ** p2);
   }
 }
 ```
@@ -105,13 +129,17 @@ ghost fn split (b: bool) (p1 p2: slprop)
   ensures  if_ b p1 ** if_ b p2
 {
   if b {
-    if_elim_true b (p1 ** p2);
-    if_intro_true b p1;
-    if_intro_true b p2;
+    if_elim_true (p1 ** p2);
+    if_intro_true p1;
+    if_rewrite_bool true b p1;
+    if_intro_true p2;
+    if_rewrite_bool true b p2;
   } else {
-    if_elim_false b (p1 ** p2);
-    if_intro_false b p1;
-    if_intro_false b p2;
+    if_elim_false (p1 ** p2);
+    if_intro_false p1;
+    if_rewrite_bool false b p1;
+    if_intro_false p2;
+    if_rewrite_bool false b p2;
   }
 }
 ```
@@ -124,12 +152,12 @@ ghost fn if_map (#b: bool) (#p #q: slprop) (f: unit -> (stt_ghost unit emp_iname
   ensures  if_ b q
 {
   if b {
-    if_elim_true b p;
+    if_elim_true p;
     f ();
-    if_intro_true b q;
+    if_intro_true q;
   } else {
-    if_elim_false b p;
-    if_intro_false b q;
+    if_elim_false p;
+    if_intro_false q;
   }
 }
 ```
@@ -140,33 +168,17 @@ ghost fn if_flatten (#b1 #b2: bool) (#p: slprop)
   ensures  if_ (b1 && b2) p
 {
   if b1 {
-    if_elim_true b1 (if_ b2 p);
+    if_elim_true (if_ b2 p);
     if b2 {
-      if_elim_true b2 p;
-      if_intro_true (b1 && b2) p;
+      if_elim_true  p;
+      if_intro_true p;
     } else {
-      if_elim_false b2 p;
-      if_intro_false (b1 && b2) p;
+      if_elim_false p;
+      if_intro_false p;
     }
   } else {
-    if_elim_false b1 (if_ b2 p);
-    if_intro_false (b1 && b2) p;
-  }
-}
-```
-
-// REWRITE
-
-```pulse
-ghost fn if_rewrite (#b: bool) (#p1 p2: slprop) (#e: (squash b -> squash (p1 == p2)))
-  requires if_ b p1
-  ensures  if_ b p2
-{
-  if b {
-    e ();
-    rewrite each p1 as p2;
-  } else {
-    ()
+    if_elim_false (if_ b2 p);
+    if_intro_false p;
   }
 }
 ```
@@ -186,25 +198,21 @@ ghost fn bigstar_if_elim
   ensures  p x
 {
   bigstar_extract m n _ x;
-  bigstar_map
-    #u1 #u1
-    #m #x
-    #(fun (i: nat { m <= i /\ i < x }) -> _ i)
-    #(fun _ -> emp)
-    (fun (i: nat { m <= i /\ i < x }) ->
-      if_elim_false ((i <: nat) = x) (p (i <: nat)));
+
+  bigstar_map #u1 #u1 #m #x
+    (fun (i: nat { m <= i /\ i < x }) -> if_rewrite_bool ((i <: nat) = x) false (p (i <: nat)));
+  bigstar_map #u1 #u1 #m #x
+    (fun (i: nat { m <= i /\ i < x }) -> if_elim_false (p (i <: nat)));
 
   bigstar_emp_elim #_ #m #x;
-  bigstar_map
-    #u1 #u1
-    #(x + 1) #n
-    #(fun (i: nat {(x+1) <= i /\ i < n }) -> _ i)
-    #(fun _ -> emp)
-    (fun (i: nat { (x + 1) <= i /\ i < n }) ->
-      if_elim_false ((i <: nat) = x) (p (i <: nat)));
+
+  bigstar_map #u1 #u1 #(x + 1) #n
+    (fun (i: nat { (x + 1) <= i /\ i < n }) -> if_rewrite_bool ((i <: nat) = x) false (p (i <: nat)));
+  bigstar_map #u1 #u1 #(x + 1) #n
+    (fun (i: nat { (x + 1) <= i /\ i < n }) -> if_elim_false (p (i <: nat)));
 
   bigstar_emp_elim #_ #(x + 1) #n;
-  if_elim_true true (p x)
+  if_elim_true (p x)
 }
 ```
 
@@ -219,13 +227,17 @@ fn __bigstar_if_intro
   requires p x
   ensures  bigstar #u1 m n (fun (i:nat { m <= i /\ i < n }) -> if_ (op_Equality #nat i x) (p i))
 {
-  if_intro_true true (p x);
+  if_intro_true (p x);
   bigstar_emp_intro #u1 m x;
   bigstar_map #u1 #u1 #m #x #(fun _ -> emp) #(fun (i: nat { m <= i /\ i < x }) -> _ i) 
-    (fun (i: nat { m <= i /\ i < x }) -> if_intro_false ((i <: nat) = x) (p (i <: nat)));
+    (fun (i: nat { m <= i /\ i < x }) -> if_intro_false (p (i <: nat)));
+  bigstar_map #u1 #u1 #m #x #(fun _ -> emp) #(fun (i: nat { m <= i /\ i < x }) -> _ i) 
+    (fun (i: nat { m <= i /\ i < x }) -> if_rewrite_bool false ((i <: nat) = x) (p (i <: nat)));
   bigstar_emp_intro #u1 (x + 1) n;
   bigstar_map #u1 #u1 #(x + 1) #n #(fun _ -> emp) #(fun (i: nat { (x + 1) <= i /\ i < n }) -> _ i) 
-    (fun (i: nat { (x + 1) <= i /\ i < n }) -> if_intro_false ((i <: nat) = x) (p (i <: nat)));
+    (fun (i: nat { (x + 1) <= i /\ i < n }) -> if_intro_false (p (i <: nat)));
+  bigstar_map #u1 #u1 #(x + 1) #n #(fun _ -> emp) #(fun (i: nat { (x + 1) <= i /\ i < n }) -> _ i) 
+    (fun (i: nat { (x + 1) <= i /\ i < n }) -> if_rewrite_bool false ((i <: nat) = x) (p (i <: nat)));
   bigstar_compose #u1 m n (fun (i:nat { m <= i /\ i < n }) -> if_ (op_Equality #nat i x) (p i)) x;
 }
 ```
