src/lib/GPU.MatrixBarrier.fsti
@@ -5,14 +5,15 @@ open Pulse.Lib.BigStar
 open FStar.Tactics.V2
 open GPU.Base
 module B = GPU.Barrier2
+open GPU.SizeT
+module SZ = FStar.SizeT
 
 let mbarrier_tok
-  (#n:nat)
+  (n:nat)
   (p : (it:nat -> from: nat { 0 <= from /\ from < n } -> to: nat { 0 <= to /\ to < n } -> slprop))
-  (b : B.barrier n)
   (it : nat)
   (tid : nat { 0 <= tid /\ tid < n })
-  : slprop = B.barrier_tok #n
+  : slprop = exists* b. B.barrier_tok #n
     (fun it (from : nat { 0 <= from /\ from < n }) -> bigstar 0 n (p it from))
     (fun it (to : nat { 0 <= to /\ to < n }) -> bigstar 0 n (fun (from : nat { 0 <= from /\ from < n }) -> p it from to)) b it tid
 
@@ -42,27 +43,25 @@ ghost fn fold_mbarrier_tok
   requires B.barrier_tok #n
     (fun it (from : nat { 0 <= from /\ from < n }) -> bigstar 0 n (p it from))
     (fun it (to : nat { 0 <= to /\ to < n }) -> bigstar 0 n (fun (from : nat { 0 <= from /\ from < n }) -> p it from to)) b it tid
-  ensures mbarrier_tok #n p b it tid
+  ensures mbarrier_tok n p it tid
 {
-  fold (mbarrier_tok #n p b it tid)
+  fold (mbarrier_tok n p it tid)
 }
 ```
 
 ```pulse
 ghost
 fn mk_mbarrier
-  (n : nat)
+  (n: SZ.t { 0 < n /\ n <= max_threads })
   (p : (it:nat -> from: nat { 0 <= from /\ from < n } -> to: nat { 0 <= to /\ to < n } -> slprop))
-  requires emp
-  returns  b : erased (B.barrier n)
-  ensures  bigstar 0 n (mbarrier_tok p b 0)
+  requires block_setup n
+  ensures  block_setup n ** bigstar 0 n (mbarrier_tok n p 0)
 {
   let b = B.mk_barrier n
     (fun it (from : nat { 0 <= from /\ from < n }) -> bigstar 0 n (p it from))
     (fun it (to : nat { 0 <= to /\ to < n }) -> bigstar 0 n (fun (from : nat { 0 <= from /\ from < n }) -> p it from to))
     (mk_mbarrier_proof n p);
   bigstar_map #0 #0 #0 #n (fold_mbarrier_tok #n p b 0);
-  b
 }
 ```
 
@@ -71,15 +70,14 @@ fn mk_mbarrier
 fn mbarrier_wait
   (#n : erased nat)
   (#p : (it:nat -> from: nat { 0 <= from /\ from < n } -> to: nat { 0 <= to /\ to < n } -> slprop))
-  (b : B.barrier n)
   (#it : erased nat)
   (#tid : erased nat { tid < n })
-  requires mbarrier_tok p b  it    tid ** bigstar 0 n (p it tid)
-  ensures  mbarrier_tok p b (it+1) tid ** bigstar 0 n (fun (from: nat { 0 <= from /\ from < n }) -> p it from tid)
+  requires mbarrier_tok n p  it    tid ** bigstar 0 n (p it tid)
+  ensures  mbarrier_tok n p (it+1) tid ** bigstar 0 n (fun (from: nat { 0 <= from /\ from < n }) -> p it from tid)
 {
   unfold mbarrier_tok;
-  B.barrier_wait #n #(fun it (from: nat { 0 <= from /\ from < n }) -> bigstar 0 n (p it from)) #_ b;
-  fold (mbarrier_tok p b (it+1) tid);
+  B.barrier_wait #n #(fun it (from: nat { 0 <= from /\ from < n }) -> bigstar 0 n (p it from)) #_ _;
+  fold (mbarrier_tok n p (it+1) tid);
 }
 ```
 
@@ -89,9 +87,8 @@ val
 fn drop_mbarrier
   (#n : nat)
   (#p : (it:nat -> from: nat { from < n } -> to: nat { to < n } -> slprop))
-  (#b : B.barrier n)
   (#it: nat)
-  requires bigstar 0 n (mbarrier_tok p b it)
+  requires bigstar 0 n (mbarrier_tok n p it)
   ensures  emp
 ```
 
