src/examples/matmul/GPU.MatMul.Defs.fsti
@@ -1,5 +1,5 @@
 module GPU.MatMul.Defs
 
 include GPU.MatMul.Kernel
-include GPU.MatMul.Pure
 include GPU.MatMul.Impure
+include GPU.MatMul.Pure
