src/lib/GPU.Kernel.fsti
@@ -10,28 +10,48 @@ open GPU.Base
 open GPU.MatrixBarrier
 open FStar.Mul
 module U32 = FStar.UInt32
+module SZ = FStar.SizeT
 
 (* f<<<nblk, nthr>>>(...); *)
 ```pulse
 val
 fn launch_kernel_n_m_sync
   (#u1: erased int)
-  (nblk : U32.t { 0 < nblk /\ nblk <= max_blocks })
-  (nthr : U32.t { 0 < nthr /\ nthr <= max_threads })
+  (nblk : SZ.t { 0 < nblk /\ nblk <= max_blocks })
+  (nthr : SZ.t { 0 < nthr /\ nthr <= max_threads })
   (#pre #post : (tid:nat{ 0 <= tid /\ tid < (nblk * nthr) } -> slprop))
 
-  (barrier : (it:nat -> from: nat { 0 <= from /\ from < nthr } -> to: nat { 0 <= to /\ to < nthr } -> slprop))
-  (smem_sz : U32.t)
-  (smem : (to: nat { 0 <= to /\ to < nthr } -> slprop))
-  (smem_split :
-    (ar: gpu_array U32.t smem_sz) -> (v: FStar.Seq.seq U32.t) ->
+  (smem_sz : SZ.t)
+  (#shared_pre : (ar: gpu_array U32.t smem_sz) -> (tid: nat { 0 <= tid /\ tid < nthr } -> slprop))
+  (#shared_post : (ar: gpu_array U32.t smem_sz) -> (tid: nat { 0 <= tid /\ tid < nthr } -> slprop))
+  (setup : (ar: gpu_array U32.t smem_sz) -> (bid: SZ.t { 0 <= bid /\ bid < nblk }) ->
     stt_ghost unit emp_inames
-      (gpu_pts_to_array #U32.t #smem_sz ar #1.0R v) (fun _ -> bigstar 0 nthr smem))
+      (block_setup nthr ** (exists* v. gpu_pts_to_array #U32.t #smem_sz ar #1.0R v))
+      (fun _ -> block_setup nthr ** bigstar 0 nthr (shared_pre ar)))
 
   (k :
-    (b : erased (GPU.Barrier2.barrier nthr)) -> (etid: erased tid_t { gdim_x etid == nblk /\ bdim_x etid == nthr }) ->
-    stt unit (         gpu ** thread_id etid ** smem (tidx_x etid) ** mbarrier_tok barrier b 0 (tidx_x etid) ** pre (thread_index etid))
-             (fun _ -> gpu ** thread_id etid ** smem (tidx_x etid) ** mbarrier_tok barrier b 0 (tidx_x etid) ** post (thread_index etid))
+    (ar: gpu_array U32.t smem_sz) -> (etid: erased tid_t { gdim_x etid == nblk /\ bdim_x etid == nthr }) ->
+    stt unit (         gpu ** thread_id etid ** shared_pre ar (tidx_x etid) ** pre (thread_index etid))
+             (fun _ -> gpu ** thread_id etid ** shared_post ar (tidx_x etid) ** post (thread_index etid))
+  )
+  requires cpu ** bigstar #u1 0 (nblk * nthr) pre
+  ensures  cpu ** bigstar #u1 0 (nblk * nthr) post
+```
+
+(* f<<<nblk, nthr>>>(...); *)
+```pulse
+val
+fn launch_kernel_n_m_barrier
+  (#u1: erased int)
+  (nblk : SZ.t { 0 < nblk /\ nblk <= max_blocks })
+  (nthr : SZ.t { 0 < nthr /\ nthr <= max_threads })
+  (#pre #post : (tid:nat{ 0 <= tid /\ tid < (nblk * nthr) } -> slprop))
+
+  (#p: (it:nat -> from: nat { 0 <= from /\ from < nthr } -> to: nat { 0 <= to /\ to < nthr } -> slprop))
+  (k :
+    (etid: erased tid_t { gdim_x etid == nblk /\ bdim_x etid == nthr }) ->
+    stt unit (         gpu ** thread_id etid ** mbarrier_tok nthr p 0 (tidx_x etid) ** pre (thread_index etid))
+             (fun _ -> gpu ** thread_id etid ** (exists* it. mbarrier_tok nthr p it (tidx_x etid)) ** post (thread_index etid))
   )
   requires cpu ** bigstar #u1 0 (nblk * nthr) pre
   ensures  cpu ** bigstar #u1 0 (nblk * nthr) post
@@ -42,8 +62,8 @@ fn launch_kernel_n_m_sync
 val
 fn launch_kernel_n_m
   (#u1: erased int)
-  (nblk : U32.t { 0 < nblk /\ nblk <= max_blocks })
-  (nthr : U32.t { 0 < nthr /\ nthr <= max_threads })
+  (nblk : SZ.t { 0 < nblk /\ nblk <= max_blocks })
+  (nthr : SZ.t { 0 < nthr /\ nthr <= max_threads })
   (#pre #post : (tid:nat{ 0 <= tid /\ tid < (nblk * nthr) } -> slprop))
   (k :
     (etid: erased tid_t { gdim_x etid == nblk /\ bdim_x etid == nthr }) ->
@@ -58,14 +78,14 @@ fn launch_kernel_n_m
 ```pulse
 // Private
 fn kernel_n_as_n_m
-  (nblk  : U32.t { 0 < nblk /\ nblk <= max_blocks })
-  (#pre #post : (tid:nat{ 0 <= tid /\ tid < U32.v nblk } -> slprop))
+  (nblk  : SZ.t { 0 < nblk /\ nblk <= max_blocks })
+  (#pre #post : (tid:nat{ 0 <= tid /\ tid < SZ.v nblk } -> slprop))
   (k :
-    (etid:erased tid_t { gdim_x etid == nblk /\ bdim_x etid == 1ul }) ->
+    (etid:erased tid_t { gdim_x etid == nblk /\ bdim_x etid == 1sz }) ->
     stt unit (gpu ** thread_id etid ** pre (thread_index etid))
              (fun _ -> gpu ** thread_id etid ** post (thread_index etid))
   )
-  (etid:erased tid_t { gdim_x etid == nblk /\ bdim_x etid == 1ul })
+  (etid:erased tid_t { gdim_x etid == nblk /\ bdim_x etid == 1sz })
   requires gpu ** thread_id etid ** pre (thread_index etid)
   ensures  gpu ** thread_id etid ** post (thread_index etid)
 {
@@ -76,20 +96,20 @@ fn kernel_n_as_n_m
 ```pulse
 fn launch_kernel_n
   (#u1: erased int)
-  (nblk  : U32.t { 0 < nblk /\ nblk <= max_blocks })
-  (#pre #post : (tid:nat{ 0 <= tid /\ tid < U32.v nblk } -> slprop))
+  (nblk  : SZ.t { 0 < nblk /\ nblk <= max_blocks })
+  (#pre #post : (tid:nat{ 0 <= tid /\ tid < SZ.v nblk } -> slprop))
   (k :
-    (etid:erased tid_t { gdim_x etid == nblk /\ bdim_x etid == 1ul }) ->
+    (etid:erased tid_t { gdim_x etid == nblk /\ bdim_x etid == 1sz }) ->
     stt unit (gpu ** thread_id etid ** pre (thread_index etid))
              (fun _ -> gpu ** thread_id etid ** post (thread_index etid))
   )
-  requires cpu ** bigstar #u1 0 (U32.v nblk) pre
-  ensures  cpu ** bigstar #u1 0 (U32.v nblk) post
+  requires cpu ** bigstar #u1 0 (SZ.v nblk) pre
+  ensures  cpu ** bigstar #u1 0 (SZ.v nblk) post
 {
-  rewrite (bigstar #u1 0 (U32.v nblk) pre) as (bigstar #u1 0 (U32.v nblk * 1) pre);
-  launch_kernel_n_m #u1 nblk 1ul #pre #post
+  rewrite (bigstar #u1 0 (SZ.v nblk) pre) as (bigstar #u1 0 (SZ.v nblk * 1) pre);
+  launch_kernel_n_m #u1 nblk 1sz #pre #post
     (fun etid -> kernel_n_as_n_m nblk #pre #post k etid);
-  rewrite (bigstar #u1 0 (U32.v nblk * 1) post) as (bigstar #u1 0 (U32.v nblk) post);
+  rewrite (bigstar #u1 0 (SZ.v nblk * 1) post) as (bigstar #u1 0 (SZ.v nblk) post);
 }
 ```
 
@@ -101,7 +121,7 @@ fn kernel_1_as_n
   (k : unit ->
     stt unit (gpu ** pre) (fun _ -> gpu ** post)
   )
-  (etid:erased tid_t { gdim_x etid == 1ul /\ bdim_x etid == 1ul })
+  (etid:erased tid_t { gdim_x etid == 1sz /\ bdim_x etid == 1sz })
   requires gpu ** thread_id etid ** pre
   ensures  gpu ** thread_id etid ** post
 {
@@ -119,7 +139,7 @@ fn launch_kernel_1
   ensures  cpu ** post
 {
   bigstar_single_intro 0 (fun (i: nat { 0 <= i /\ i < 1 }) -> pre);
-  launch_kernel_n 1ul (fun etid -> kernel_1_as_n #pre #post k etid);
+  launch_kernel_n 1sz (fun etid -> kernel_1_as_n #pre #post k etid);
   bigstar_single_elim #0;
 }
 ```
